.

pure/MyUtilities.v
@@ -1551,6 +1551,8 @@ Module MyUtilities.
 
   End ACKERMANN.
 
+  Section FIBONACCI.
+
   Lemma n_ne_S_plus_m_n :
     forall m : nat,
     forall n : nat,
@@ -1562,20 +1564,43 @@ Module MyUtilities.
     apply le_intro_S_n_le_S_m, le_intro_plus2.
   Defined.
 
-  Definition fibonacci : nat -> nat.
+  Inductive fibonacci_spec : nat -> nat -> Prop :=
+  | FibonacciSpec1 :
+    fibonacci_spec 0 0
+  | FibonacciSpec2 :
+    fibonacci_spec 1 1
+  | FibonacciSpec3 :
+    forall n : nat,
+    forall f_n : nat,
+    forall f_S_n : nat,
+    fibonacci_spec n f_n ->
+    fibonacci_spec (S n) f_S_n ->
+    fibonacci_spec (S (S n)) (f_n + f_S_n)
+  .
+
+  Definition fibonacci :
+    forall n : nat,
+    {f_n : nat | fibonacci_spec n f_n}.
   Proof.
-    apply accumulation_leq with (phi := fun _ => nat).
+    apply accumulation_leq with (phi := fun n : nat => {f_n : nat | fibonacci_spec n f_n}).
     intros n acc.
     destruct n as [| [| n'']].
     - set (f_0 := 0).
-      exact f_0.
+      exists f_0.
+      constructor 1.
     - set (f_1 := 1).
-      exact f_1.
-    - set (f_n'' := acc n'' (leq_step n'' (S n'') (leq_step n'' n'' (leq_init n''))) (n_ne_S_plus_m_n 1 n'')).
-      set (f_n' := acc (S n'') (leq_step (S n'') (S n'') (leq_init (S n''))) (n_ne_S_plus_m_n 0 (S n''))).
+      exists f_1.
+      constructor 2.
+    - set (acc_n'' := acc n'' (leq_step n'' (S n'') (leq_step n'' n'' (leq_init n''))) (n_ne_S_plus_m_n 1 n'')).
+      set (f_n'' := proj1_sig acc_n'').
+      set (acc_n' := acc (S n'') (leq_step (S n'') (S n'') (leq_init (S n''))) (n_ne_S_plus_m_n 0 (S n''))).
+      set (f_n' := proj1_sig acc_n').
       set (f_n := f_n'' + f_n').
-      exact f_n.
+      exists f_n.
+      constructor 3; [exact (proj2_sig acc_n'') | exact (proj2_sig acc_n')].
   Defined.
+
+  End FIBONACCI.
 
 End MyUtilities.
 
